MonadicHHL/Instances/OptionT.lean
@@ -2,6 +2,11 @@ import MonadicHHL.HHLMonads
 import MonadicHHL.HHLWithVal
 import MonadicHHL.Instances.Id
 
+def optionify {α β : Type _} {m : Type _ → Type _} [Monad m]
+  (f : α → m (Option β)) : Option α → m (Option β)
+  | some a => f a
+  | none   => pure n
+
 open HHL
 ------------ OptionT ---------------
 
